Clean-up of composition and backlifting theories + libraries

src/tools/backlifter/bir_backlifterLib.sml
@@ -45,10 +45,10 @@ fun get_arm8_contract_sing bir_ct prog_bin arm8_pre arm8_post bir_prog_def bir_p
   let
     val word_from_address = bir_immSyntax.dest_Imm64 o bir_programSyntax.dest_BL_Address
 
-    val bir_prog = get_bir_simp_jgmt_prog bir_ct
+    val bir_prog = get_bir_cont_prog bir_ct
     val l =
-      word_from_address (get_bir_simp_jgmt_start_label bir_ct)
-    val ls = pred_setSyntax.mk_set (map word_from_address (pred_setSyntax.strip_set (get_bir_simp_jgmt_wlist bir_ct)))
+      word_from_address (get_bir_cont_start_label bir_ct)
+    val ls = pred_setSyntax.mk_set (map word_from_address (pred_setSyntax.strip_set (get_bir_cont_ilist bir_ct)))
     (* TODO: Note that the proof below assumes ls is a singleton *)
     val ls_sing = el 1 (pred_setSyntax.strip_set ls)
 
@@ -59,8 +59,8 @@ fun get_arm8_contract_sing bir_ct prog_bin arm8_pre arm8_post bir_prog_def bir_p
 	      ls,
 	      (((el 2) o snd o strip_comb o concl) bir_is_lifted_prog_thm),
 	      arm8_pre, arm8_post,
-	      get_bir_simp_jgmt_pre bir_ct,
-	      get_bir_simp_jgmt_post bir_ct] lift_contract_thm;
+	      get_bir_cont_pre bir_ct,
+	      get_bir_cont_post bir_ct] lift_contract_thm;
 
     (* Prove the ARM triple by supplying the antecedents of lift_contract_thm *)
     val arm8_contract_thm = prove(
@@ -78,7 +78,7 @@ fun get_arm8_contract_sing bir_ct prog_bin arm8_pre arm8_post bir_prog_def bir_p
 
       (* 2. Starting address exists in program *)
       FULL_SIMP_TAC std_ss
-	[EVAL ``MEM (^(get_bir_simp_jgmt_start_label bir_ct))
+	[EVAL ``MEM (^(get_bir_cont_start_label bir_ct))
 		    (bir_labels_of_program ^(bir_prog))``],
 
       (* 3. Provide translation of the ARM8 precondition to the BIR precondition *)
