src/tools/comp/bir_compositionLib.sml
@@ -38,16 +38,16 @@ open bir_inst_liftingHelpersLib;
     fun get_contract_post contract_thm = ((el 5) o snd o strip_comb o concl) contract_thm;
 
     (* These functions obtains the parameters of a
-     * bir_simp_jgmt *)
-    fun get_bir_simp_jgmt_prog map_triple = ((el 1) o snd o strip_comb o concl) map_triple;
-    fun get_bir_simp_jgmt_invariant map_triple = ((el 2) o snd o strip_comb o concl) map_triple;
-    fun get_bir_simp_jgmt_start_label map_triple = ((el 3) o snd o strip_comb o concl) map_triple;
-    fun get_bir_simp_jgmt_wlist map_triple = ((el 4) o snd o strip_comb o concl) map_triple;
-    fun get_bir_simp_jgmt_blist map_triple = ((el 5) o snd o strip_comb o concl) map_triple;
-    fun get_bir_simp_jgmt_pre map_triple = ((el 6) o snd o strip_comb o concl) map_triple;
-    fun get_bir_simp_jgmt_post map_triple = ((el 7) o snd o strip_comb o concl) map_triple;
+     * bir_cont *)
+    fun get_bir_cont_prog bir_cont_thm = ((el 1) o snd o strip_comb o concl) bir_cont_thm;
+    fun get_bir_cont_invariant bir_cont_thm = ((el 2) o snd o strip_comb o concl) bir_cont_thm;
+    fun get_bir_cont_start_label bir_cont_thm = ((el 3) o snd o strip_comb o concl) bir_cont_thm;
+    fun get_bir_cont_ilist bir_cont_thm = ((el 4) o snd o strip_comb o concl) bir_cont_thm;
+    fun get_bir_cont_elist bir_cont_thm = ((el 5) o snd o strip_comb o concl) bir_cont_thm;
+    fun get_bir_cont_pre bir_cont_thm = ((el 6) o snd o strip_comb o concl) bir_cont_thm;
+    fun get_bir_cont_post bir_cont_thm = ((el 7) o snd o strip_comb o concl) bir_cont_thm;
 
-    fun bir_simp_jgmt_tm_get_sort_ls_thm ct_tm =
+    fun bir_cont_tm_get_sort_ls_thm ct_tm =
       let
 	val ls = ((el 4) o snd o strip_comb) ct_tm
 	val sorted_ls =
@@ -69,18 +69,18 @@ open bir_inst_liftingHelpersLib;
     fun remove_foralls t = (remove_foralls o snd o dest_forall) t
                            handle HOL_ERR _ => t;
 
-    fun use_pre_str_rule_simp simp_ct_thm pre_impl_wp =
+    fun use_pre_str_rule_simp bir_cont_thm pre_impl_wp =
       let
-	val simp_ct_thm = SIMP_RULE std_ss [bir_bool_expTheory.bir_exp_and_def] simp_ct_thm;
+	val bir_cont_thm = SIMP_RULE std_ss [bir_bool_expTheory.bir_exp_and_def] bir_cont_thm;
         val pre_wo = (remove_foralls o concl) pre_impl_wp;
 	val pre = ((el 2) o snd o strip_comb o (el 2) o snd o strip_comb o hd o snd o strip_comb) pre_wo;
-	val prog = get_bir_simp_jgmt_prog simp_ct_thm;
-        val invar = get_bir_simp_jgmt_invariant simp_ct_thm;
-	val entry = get_bir_simp_jgmt_start_label simp_ct_thm;
-	val wlist = get_bir_simp_jgmt_wlist simp_ct_thm;
-	val blist = get_bir_simp_jgmt_blist simp_ct_thm;
-	val post = get_bir_simp_jgmt_post simp_ct_thm;
-	val wp = get_bir_simp_jgmt_pre simp_ct_thm;
+	val prog = get_bir_cont_prog bir_cont_thm;
+        val invar = get_bir_cont_invariant bir_cont_thm;
+	val entry = get_bir_cont_start_label bir_cont_thm;
+	val ilist = get_bir_cont_ilist bir_cont_thm;
+	val elist = get_bir_cont_elist bir_cont_thm;
+	val post = get_bir_cont_post bir_cont_thm;
+	val wp = get_bir_cont_pre bir_cont_thm;
         val taut_eq_thm = computeLib.RESTR_EVAL_CONV [(fst o strip_comb) pre, ``bir_exp_is_taut``] (concl pre_impl_wp);
 	val taut_thm = EQ_MP taut_eq_thm pre_impl_wp;
         (* TODO: This is slow. Replace it with something faster later. *)
@@ -99,28 +99,28 @@ open bir_inst_liftingHelpersLib;
 	   (SIMP_TAC vars_ss
 	   ) [bir_valuesTheory.BType_Bool_def]
 	);
-	val new_contract_thm = ((SIMP_RULE std_ss [simp_ct_thm, taut_thm, taut_eq_thm,
+	val new_contract_thm = ((SIMP_RULE std_ss [bir_cont_thm, taut_thm, taut_eq_thm,
                                                    pre_impl_wp, wp_var_thm, pre_var_thm]) 
-	  ((ISPECL [prog, invar, entry, wlist, blist, wp, pre, post])
-	      bir_wm_instTheory.bir_simp_taut_pre_str_rule_thm)
+	  ((ISPECL [prog, invar, entry, ilist, elist, wp, pre, post])
+	      bir_tsTheory.bir_taut_pre_str_rule_thm)
 	      );
       in
         new_contract_thm
       end;
 
-    fun use_post_weak_rule_simp simp_ct_thm l2 post1_impl_post2 =
+    fun use_post_weak_rule_simp bir_cont_thm l2 post1_impl_post2 =
       let
-	val simp_ct_thm = SIMP_RULE std_ss [bir_bool_expTheory.bir_exp_and_def] simp_ct_thm;
+	val bir_cont_thm = SIMP_RULE std_ss [bir_bool_expTheory.bir_exp_and_def] bir_cont_thm;
         val post2e_wo = (remove_foralls o concl) post1_impl_post2;
 	val post2e = ((el 3) o snd o strip_comb o hd o snd o strip_comb) post2e_wo;
-	val prog = get_bir_simp_jgmt_prog simp_ct_thm;
-        val invar = get_bir_simp_jgmt_invariant simp_ct_thm;
-	val entry = get_bir_simp_jgmt_start_label simp_ct_thm;
-	val wlist = get_bir_simp_jgmt_wlist simp_ct_thm;
-	val blist = get_bir_simp_jgmt_blist simp_ct_thm;
-	val post1 = get_bir_simp_jgmt_post simp_ct_thm;
+	val prog = get_bir_cont_prog bir_cont_thm;
+        val invar = get_bir_cont_invariant bir_cont_thm;
+	val entry = get_bir_cont_start_label bir_cont_thm;
+	val ilist = get_bir_cont_ilist bir_cont_thm;
+	val elist = get_bir_cont_elist bir_cont_thm;
+	val post1 = get_bir_cont_post bir_cont_thm;
         val post2 = ``\l. if l = ^l2 then ^post2e else ^post1 l``;
-	val pre = get_bir_simp_jgmt_pre simp_ct_thm;
+	val pre = get_bir_cont_pre bir_cont_thm;
         val taut_eq_thm = computeLib.RESTR_EVAL_CONV [(fst o strip_comb) post2e, ``bir_exp_is_taut``] (concl post1_impl_post2);
 	val taut_thm = EQ_MP taut_eq_thm post1_impl_post2;
         (* TODO: This is slow. Replace it with something faster later. *)
@@ -140,39 +140,39 @@ open bir_inst_liftingHelpersLib;
 	   ) [bir_valuesTheory.BType_Bool_def]
 	);
 	val new_contract_thm = ((SIMP_RULE (std_ss++HolBACoreSimps.bir_TYPES_ss++wordsLib.WORD_ss)
-                                           [simp_ct_thm, taut_thm, taut_eq_thm,
+                                           [bir_cont_thm, taut_thm, taut_eq_thm,
                                             post1_impl_post2, post1_var_thm, post2_var_thm]) 
-	  ((ISPECL [prog, invar, entry, wlist, l2, blist, pre, post1, post2])
-	      bir_wm_instTheory.bir_simp_taut_post_weak_rule_thm)
+	  ((ISPECL [prog, invar, entry, ilist, l2, elist, pre, post1, post2])
+	      bir_tsTheory.bir_taut_post_weak_rule_thm)
 	      );
       in
         new_contract_thm
       end;
 
-    fun bir_remove_labels_from_wlist
-      not_empty_set_repr ct new_wlist =
+    fun bir_remove_labels_from_ilist
+      not_empty_set_repr ct new_ilist =
       let
-	val prog = get_bir_simp_jgmt_prog ct
-	val start_label = get_bir_simp_jgmt_start_label ct
-	val label_set = get_bir_simp_jgmt_wlist ct
+	val prog = get_bir_cont_prog ct
+	val start_label = get_bir_cont_start_label ct
+	val label_set = get_bir_cont_ilist ct
 	val to_remove_label_set = 
 	  pred_setSyntax.mk_set (
-	    filter (fn tm => not (exists (term_eq tm) (pred_setSyntax.strip_set new_wlist)))
+	    filter (fn tm => not (exists (term_eq tm) (pred_setSyntax.strip_set new_ilist)))
 		   (pred_setSyntax.strip_set label_set)
 	  )
-	val precondition = get_bir_simp_jgmt_pre ct
-	val postcondition = get_bir_simp_jgmt_post ct
+	val precondition = get_bir_cont_pre ct
+	val postcondition = get_bir_cont_post ct
 
 	val bir_spec_subset_rule_thm =
 	  ISPECL [prog,
 		  start_label,
-		  new_wlist,
+		  new_ilist,
 		  to_remove_label_set,
 		  precondition,
-		  postcondition] bir_wm_instTheory.bir_simp_wl_subset_rule_thm
+		  postcondition] bir_tsTheory.bir_il_subset_rule_thm
 
 	val bir_spec_subset_rule_thm1 =
-	  (HO_MATCH_MP bir_spec_subset_rule_thm (not_empty_set_repr new_wlist))
+	  (HO_MATCH_MP bir_spec_subset_rule_thm (not_empty_set_repr new_ilist))
 
 	val removal_ante_thm =
 	  prove ((fst o dest_imp o concl) bir_spec_subset_rule_thm1,
@@ -193,7 +193,7 @@ open bir_inst_liftingHelpersLib;
 	  )
 
 	  val bir_spec_subset_rule_thm2 =
-	    (fn thm => ONCE_REWRITE_RULE [bir_simp_jgmt_tm_get_sort_ls_thm
+	    (fn thm => ONCE_REWRITE_RULE [bir_cont_tm_get_sort_ls_thm
 					    ((fst o dest_imp o concl) thm)] thm
 	    )
 	    (SIMP_RULE (std_ss++HolBACoreSimps.bir_union_var_set_ss) []
@@ -202,7 +202,7 @@ open bir_inst_liftingHelpersLib;
 
 	  val bir_spec_subset_rule_thm3 =
 	    HO_MATCH_MP bir_spec_subset_rule_thm2
-	     ((fn thm => ONCE_REWRITE_RULE [bir_simp_jgmt_tm_get_sort_ls_thm (concl thm)] thm)
+	     ((fn thm => ONCE_REWRITE_RULE [bir_cont_tm_get_sort_ls_thm (concl thm)] thm)
 		ct
 	     )
       in
@@ -210,36 +210,36 @@ open bir_inst_liftingHelpersLib;
       end
     ;
 
-    (* This function applies bir_simp_bl_subset_rule_thm
+    (* This function applies bir_el_subset_rule_thm
      * to a contract, given a set of labels to remove from the
-     * blacklist *)
-    fun bir_remove_labels_from_blist (simp_in_set_repr_tac) map_ct to_remove_from_blist =
+     * exclude list *)
+    fun bir_remove_labels_from_elist (simp_in_set_repr_tac) map_ct to_remove_from_elist =
       let
-	val prog = get_bir_simp_jgmt_prog map_ct
-        val invariant = get_bir_simp_jgmt_invariant map_ct
-	val start_label = get_bir_simp_jgmt_start_label map_ct
-        val wlist = get_bir_simp_jgmt_wlist map_ct
-        val blist = get_bir_simp_jgmt_blist map_ct
+	val prog = get_bir_cont_prog map_ct
+        val invariant = get_bir_cont_invariant map_ct
+	val start_label = get_bir_cont_start_label map_ct
+        val ilist = get_bir_cont_ilist map_ct
+        val elist = get_bir_cont_elist map_ct
         (* TODO: Parametrize this over different set representations *)
-        val new_blist_sml =
-          filter (fn tm => not (exists (term_eq tm) (pred_setSyntax.strip_set to_remove_from_blist)))
-		 (pred_setSyntax.strip_set blist)
-	val new_blist =
-          if null new_blist_sml
+        val new_elist_sml =
+          filter (fn tm => not (exists (term_eq tm) (pred_setSyntax.strip_set to_remove_from_elist)))
+		 (pred_setSyntax.strip_set elist)
+	val new_elist =
+          if null new_elist_sml
           then pred_setSyntax.mk_empty bir_label_t_ty
-	  else pred_setSyntax.mk_set new_blist_sml
-	val precondition = get_bir_simp_jgmt_pre map_ct
-	val postcondition = get_bir_simp_jgmt_post map_ct
+	  else pred_setSyntax.mk_set new_elist_sml
+	val precondition = get_bir_cont_pre map_ct
+	val postcondition = get_bir_cont_post map_ct
 
       val bir_spec_subset_rule_thm =
 	ISPECL [prog,
                 invariant,
                 start_label,
-                wlist,
-		blist,
-		new_blist,
+                ilist,
+		elist,
+		new_elist,
 		precondition,
-		postcondition] bir_wm_instTheory.bir_simp_bl_subset_rule_thm
+		postcondition] bir_tsTheory.bir_el_subset_rule_thm
 
       val bir_spec_subset_rule_thm2 =
 	SIMP_RULE std_ss [prove((fst o dest_imp o concl) bir_spec_subset_rule_thm,
@@ -257,15 +257,15 @@ open bir_inst_liftingHelpersLib;
     local
     fun remove_label list label = filter (fn el => not (term_eq el label)) list
 
-    fun bir_populate_blacklist' _ _ [] map_triple assmpt=
-      map_triple
-      | bir_populate_blacklist' (get_labels_from_set_repr, el_in_set_repr, delete_not_empty_set_repr,
+    fun bir_populate_elist' _ _ [] bir_cont_thm assmpt =
+      bir_cont_thm
+      | bir_populate_elist' (get_labels_from_set_repr, el_in_set_repr, delete_not_empty_set_repr,
                                  mk_set_repr, simp_delete_set_repr_rule, simp_insert_set_repr_rule) post
-                                (h::t) map_triple assmpt =
+                                (h::t) bir_cont_thm assmpt =
 	  let
             (* First, check if postcondition holds for the current label h in the list of
              * exit labels *)
-	    val elabel_post_is_false_tm = mk_comb ((get_bir_simp_jgmt_post map_triple), h)
+	    val elabel_post_is_false_tm = mk_comb ((get_bir_cont_post bir_cont_thm), h)
 	    val elabel_post_is_false_thm =
 	      SIMP_CONV (std_ss++HolBACoreSimps.holBACore_ss++wordsLib.WORD_ss)
                 [ASSUME assmpt] elabel_post_is_false_tm
@@ -275,100 +275,100 @@ open bir_inst_liftingHelpersLib;
 	  in
 	    if elabel_post_is_false
 	    then let
-                   (* Apply bir_simp_wl_to_bl_rule_thm and compute antecedents *)
-		   val new_map_triple1 =
-		     HO_MATCH_MP bir_wm_instTheory.bir_simp_wl_to_bl_rule_thm map_triple
-                   (* elabel IN wlist *)
-		   val elabel_in_wlist = el_in_set_repr h (get_bir_simp_jgmt_wlist map_triple)
-		   val new_map_triple2 =
-		     HO_MATCH_MP new_map_triple1 elabel_in_wlist
-                   (* wlist DELETE elabel <> {} *)
+                   (* Apply bir_il_to_el_rule_thm and compute antecedents *)
+		   val new_bir_cont_thm1 =
+		     HO_MATCH_MP bir_tsTheory.bir_il_to_el_rule_thm bir_cont_thm
+                   (* elabel IN ilist *)
+		   val elabel_in_ilist = el_in_set_repr h (get_bir_cont_ilist bir_cont_thm)
+		   val new_bir_cont_thm2 =
+		     HO_MATCH_MP new_bir_cont_thm1 elabel_in_ilist
+                   (* ilist DELETE elabel <> {} *)
                    val delete_elabel_notempty =
-                     delete_not_empty_set_repr h (get_bir_simp_jgmt_wlist map_triple)
-		   val new_map_triple3 =
-		     HO_MATCH_MP new_map_triple2 delete_elabel_notempty
+                     delete_not_empty_set_repr h (get_bir_cont_ilist bir_cont_thm)
+		   val new_bir_cont_thm3 =
+		     HO_MATCH_MP new_bir_cont_thm2 delete_elabel_notempty
                    (* post elabel = bir_exp_false *)
-		   val new_map_triple4 =
-		     HO_MATCH_MP new_map_triple3 (SIMP_RULE std_ss [] elabel_post_is_false_thm)
+		   val new_bir_cont_thm4 =
+		     HO_MATCH_MP new_bir_cont_thm3 (SIMP_RULE std_ss [] elabel_post_is_false_thm)
                    (* Finalize with assumption and INSERT and DELETE simplification *)
-		   val new_map_triple5 =
+		   val new_bir_cont_thm5 =
                      SIMP_RULE (std_ss++stringSimps.STRING_ss++string_ss) [ASSUME assmpt]
-		     (simp_delete_set_repr_rule new_map_triple4)
-		   val new_map_triple6 =
-		     simp_insert_set_repr_rule new_map_triple5
+		     (simp_delete_set_repr_rule new_bir_cont_thm4)
+		   val new_bir_cont_thm6 =
+		     simp_insert_set_repr_rule new_bir_cont_thm5
 		 in
-		   bir_populate_blacklist' (get_labels_from_set_repr, el_in_set_repr,
+		   bir_populate_elist' (get_labels_from_set_repr, el_in_set_repr,
                                             delete_not_empty_set_repr, mk_set_repr,
                                             simp_delete_set_repr_rule, simp_insert_set_repr_rule) post
-                                           t new_map_triple5 assmpt
+                                           t new_bir_cont_thm5 assmpt
 		 end
-	    else bir_populate_blacklist' (get_labels_from_set_repr, el_in_set_repr,
+	    else bir_populate_elist' (get_labels_from_set_repr, el_in_set_repr,
                                           delete_not_empty_set_repr, mk_set_repr,
                                           simp_delete_set_repr_rule, simp_insert_set_repr_rule) post
-                                         t map_triple assmpt
+                                         t bir_cont_thm assmpt
 	  end
     in
-      fun bir_populate_blacklist_assmpt (get_labels_from_set_repr, el_in_set_repr,
+      fun bir_populate_elist_assmpt (get_labels_from_set_repr, el_in_set_repr,
                                          delete_not_empty_set_repr, mk_set_repr,
                                          simp_delete_set_repr_rule, simp_insert_set_repr_rule)
-                                        map_triple assmpt =
-	bir_populate_blacklist'
+                                        bir_cont_thm assmpt =
+	bir_populate_elist'
 	  (get_labels_from_set_repr, el_in_set_repr, delete_not_empty_set_repr, mk_set_repr,
            simp_delete_set_repr_rule, simp_insert_set_repr_rule)
-	  (get_bir_simp_jgmt_post map_triple)
-	  (get_labels_from_set_repr (get_bir_simp_jgmt_wlist map_triple))
-	  map_triple assmpt
+	  (get_bir_cont_post bir_cont_thm)
+	  (get_labels_from_set_repr (get_bir_cont_ilist bir_cont_thm))
+	  bir_cont_thm assmpt
 
-      fun bir_populate_blacklist (get_labels_from_set_repr, el_in_set_repr,
+      fun bir_populate_elist (get_labels_from_set_repr, el_in_set_repr,
                                   delete_not_empty_set_repr, mk_set_repr,
-                                  simp_delete_set_repr_rule, simp_insert_set_repr_rule) map_triple =
-	bir_populate_blacklist'
+                                  simp_delete_set_repr_rule, simp_insert_set_repr_rule) bir_cont_thm =
+	bir_populate_elist'
 	  (get_labels_from_set_repr, el_in_set_repr, delete_not_empty_set_repr, mk_set_repr,
            simp_delete_set_repr_rule, simp_insert_set_repr_rule)
-	  (get_bir_simp_jgmt_post map_triple)
-	  (get_labels_from_set_repr (get_bir_simp_jgmt_wlist map_triple))
-	  map_triple T
+	  (get_bir_cont_post bir_cont_thm)
+	  (get_labels_from_set_repr (get_bir_cont_ilist bir_cont_thm))
+	  bir_cont_thm T
     end
     ;
 
-    (* This function translates a bir_exec_to_labels_triple to bir_simp_jgmt,
+    (* This function translates a bir_exec_to_labels_triple to bir_cont,
      * and abbreviates the precondition according to a given tautology *)
-    fun label_ct_to_simp_ct (not_empty_set_repr, get_labels_from_set_repr, el_in_set_repr, delete_not_empty_set_repr,
+    fun bir_exec_to_labels_triple_to_bir_cont (not_empty_set_repr, get_labels_from_set_repr, el_in_set_repr, delete_not_empty_set_repr,
                             mk_set_repr, simp_delete_set_repr_rule, simp_insert_set_repr_rule)
                            label_ct taut_thm =
-      bir_populate_blacklist (get_labels_from_set_repr, el_in_set_repr, delete_not_empty_set_repr,
+      bir_populate_elist (get_labels_from_set_repr, el_in_set_repr, delete_not_empty_set_repr,
                               mk_set_repr, simp_delete_set_repr_rule, simp_insert_set_repr_rule)
 	(use_pre_str_rule_simp
 	  (HO_MATCH_MP
-	    (HO_MATCH_MP bir_wm_instTheory.bir_label_jgmt_impl_weak_jgmt (not_empty_set_repr (get_contract_ls label_ct))) label_ct
+	    (HO_MATCH_MP bir_tsTheory.bir_label_jgmt_impl_weak_jgmt (not_empty_set_repr (get_contract_ls label_ct))) label_ct
 	  )
 	  taut_thm
 	)
       ;
 
-    fun label_ct_to_simp_ct_assmpt (not_empty_set_repr, get_labels_from_set_repr, el_in_set_repr, delete_not_empty_set_repr,
+    fun bir_exec_to_labels_triple_to_bir_cont_assmpt (not_empty_set_repr, get_labels_from_set_repr, el_in_set_repr, delete_not_empty_set_repr,
                                    mk_set_repr, simp_delete_set_repr_rule, simp_insert_set_repr_rule)
                                   label_ct taut_thm assmpt =
-      bir_populate_blacklist_assmpt (get_labels_from_set_repr, el_in_set_repr,
+      bir_populate_elist_assmpt (get_labels_from_set_repr, el_in_set_repr,
                                      delete_not_empty_set_repr, mk_set_repr,
 			             simp_delete_set_repr_rule, simp_insert_set_repr_rule)
 	(use_pre_str_rule_simp
 	  (HO_MATCH_MP
-            (HO_MATCH_MP bir_wm_instTheory.bir_label_jgmt_impl_weak_jgmt (not_empty_set_repr (get_contract_ls label_ct))
+            (HO_MATCH_MP bir_tsTheory.bir_label_jgmt_impl_weak_jgmt (not_empty_set_repr (get_contract_ls label_ct))
             ) (UNDISCH_ALL (SPEC_ALL label_ct))
 	  )
 	  taut_thm
 	) assmpt;
 
-    fun label_ct_to_simp_ct_no_taut_assmpt (not_empty_set_repr, get_labels_from_set_repr, el_in_set_repr,
+    fun bir_exec_to_labels_triple_to_bir_cont_no_taut_assmpt (not_empty_set_repr, get_labels_from_set_repr, el_in_set_repr,
                                            delete_not_empty_set_repr, mk_set_repr,
 			                   simp_delete_set_repr_rule, simp_insert_set_repr_rule)
                                           label_ct assmpt =
-      bir_populate_blacklist_assmpt (get_labels_from_set_repr, el_in_set_repr,
+      bir_populate_elist_assmpt (get_labels_from_set_repr, el_in_set_repr,
                                      delete_not_empty_set_repr, mk_set_repr,
 			             simp_delete_set_repr_rule, simp_insert_set_repr_rule)
 	  (HO_MATCH_MP
-            (HO_MATCH_MP bir_wm_instTheory.bir_label_jgmt_impl_weak_jgmt (not_empty_set_repr (get_contract_ls label_ct))
+            (HO_MATCH_MP bir_tsTheory.bir_label_jgmt_impl_weak_jgmt (not_empty_set_repr (get_contract_ls label_ct))
             ) (UNDISCH_ALL (SPEC_ALL label_ct))
 	  ) assmpt;
 
@@ -376,22 +376,22 @@ open bir_inst_liftingHelpersLib;
     fun bir_compose_simp_loop (simp_in_set_repr_tac, inter_set_repr_ss, union_set_repr_ss) loop_map_ct
           loop_exit_map_ct loop_invariant loop_condition loop_variant prog_def def_list = 
       let
-	(* 1. Specialise bir_simp_signed_loop_rule_thm *)
-	val prog = get_bir_simp_jgmt_prog loop_exit_map_ct
-	val start_label = get_bir_simp_jgmt_start_label loop_map_ct
-	val wlist = get_bir_simp_jgmt_wlist loop_exit_map_ct
-	val blist = get_bir_simp_jgmt_blist loop_exit_map_ct
+	(* 1. Specialise bir_signed_loop_rule_thm *)
+	val prog = get_bir_cont_prog loop_exit_map_ct
+	val start_label = get_bir_cont_start_label loop_map_ct
+	val ilist = get_bir_cont_ilist loop_exit_map_ct
+	val elist = get_bir_cont_elist loop_exit_map_ct
 
 	val bir_add_comp_while_rule_thm =
 	  ISPECL [prog,
 		  start_label,
-		  wlist,
-		  blist,
+		  ilist,
+		  elist,
 		  loop_invariant,
 		  loop_condition,
 		  loop_variant,
-		  get_bir_simp_jgmt_post loop_exit_map_ct]
-                 bir_wm_instTheory.bir_simp_signed_loop_rule_thm
+		  get_bir_cont_post loop_exit_map_ct]
+                 bir_tsTheory.bir_signed_loop_rule_thm
 
 	(* 2. Knock out antecedents:  *)
 	(* Note: This structure enforces the property that each step only touches the
@@ -429,21 +429,21 @@ open bir_inst_liftingHelpersLib;
 						                  bir_add_reg_prog_def needed *)
 				     )] bir_add_comp_while_rule_thm3
 
-	(* Start label should not be in whitelist *)
+	(* Start label should not be in include list *)
 	(* TODO: Construct this antecedent explicitly in place *)
 	val bir_add_comp_while_rule_thm5 =
 	  SIMP_RULE std_ss [prove((fst o dest_imp o concl) bir_add_comp_while_rule_thm4,
 				       simp_in_set_repr_tac
 				     )] bir_add_comp_while_rule_thm4
 
-	(* Start label should not be in blacklist *)
+	(* Start label should not be in exclude list *)
 	(* TODO: Construct this antecedent explicitly in place *)
 	val bir_add_comp_while_rule_thm6 =
 	  SIMP_RULE std_ss [prove((fst o dest_imp o concl) bir_add_comp_while_rule_thm5,
 				       simp_in_set_repr_tac
 				     )] bir_add_comp_while_rule_thm5
 
-	(* Intersection of whitelist and blacklist should be empty set *)
+	(* Intersection of include list and exclude list should be empty set *)
 	(* TODO: Construct this antecedent explicitly in place *)
 	val bir_add_comp_while_rule_thm7 =
 	  SIMP_RULE std_ss [prove((fst o dest_imp o concl) bir_add_comp_while_rule_thm6,
@@ -458,15 +458,15 @@ open bir_inst_liftingHelpersLib;
 	    GEN_TAC >>
 	    ASSUME_TAC (Q.SPEC `x` (GEN_ALL loop_map_ct)) >>
 (*
-	    FULL_SIMP_TAC std_ss [bir_wm_instTheory.bir_triple_equiv_simp_jgmt] >>
+	    FULL_SIMP_TAC std_ss [bir_tsTheory.bir_triple_equiv_simp_jgmt] >>
 *)
 	    FULL_SIMP_TAC (std_ss++inter_set_repr_ss++union_set_repr_ss) [] >>
 	    FULL_SIMP_TAC (std_ss++pred_setLib.PRED_SET_ss) [] >>
-	    FULL_SIMP_TAC std_ss [bir_wm_instTheory.bir_simp_jgmt_def,
-				  abstract_simp_hoare_logicTheory.abstract_simp_jgmt_def,
-				  abstract_hoare_logicTheory.abstract_jgmt_def,
-				  bir_wm_instTheory.bir_exec_to_labels_triple_precond_def,
-				  bir_wm_instTheory.bir_exec_to_labels_triple_postcond_def] >>
+	    FULL_SIMP_TAC std_ss [bir_tsTheory.bir_cont_def,
+				  total_ext_program_logicTheory.t_ext_jgmt_def,
+				  total_program_logicTheory.t_jgmt_def,
+				  bir_tsTheory.bir_exec_to_labels_triple_precond_def,
+				  bir_tsTheory.bir_exec_to_labels_triple_postcond_def] >>
 	    REPEAT STRIP_TAC >> (
               FULL_SIMP_TAC (std_ss++pred_setLib.PRED_SET_ss) []
             ) >>
@@ -508,10 +508,10 @@ open bir_inst_liftingHelpersLib;
               ),
 
               (* bool_exp_env of invariant *)
-	      FULL_SIMP_TAC (std_ss++abstract_hoare_logicSimps.bir_wm_SS)
-		[bir_bool_expTheory.bir_is_bool_exp_env_def, bir_wm_instTheory.bir_etl_wm_def, bir_wm_instTheory.bir_weak_trs_def] >>
+	      FULL_SIMP_TAC (std_ss++program_logicSimps.bir_wm_SS)
+		[bir_bool_expTheory.bir_is_bool_exp_env_def, bir_tsTheory.bir_ts_def, bir_tsTheory.bir_weak_trs_def] >>
               Cases_on `bir_exec_to_labels
-              (^(pred_setSyntax.mk_set [start_label]) UNION (^wlist))
+              (^(pred_setSyntax.mk_set [start_label]) UNION (^ilist))
               (bir_add_reg_prog:'observation_type bir_program_t) s` >> (
                 FULL_SIMP_TAC (std_ss++HolBACoreSimps.holBACore_ss) [bir_programTheory.bir_exec_to_labels_def]
               ) >>
@@ -537,27 +537,27 @@ open bir_inst_liftingHelpersLib;
       end
     ;
 
-    (* This function composes a loop from a looping bir_simp_jgmt
-     * and a loop exit bir_simp_jgmt *)
+    (* This function composes a loop from a looping bir_cont
+     * and a loop exit bir_cont *)
     fun bir_compose_simp_loop_unsigned (simp_in_set_repr_tac, inter_set_repr_ss, union_set_repr_ss) loop_map_ct
           loop_exit_map_ct loop_invariant loop_condition loop_variant prog_def def_list = 
       let
-	(* 1. Specialise bir_simp_unsigned_loop_rule_thm *)
-	val prog = get_bir_simp_jgmt_prog loop_exit_map_ct
-	val start_label = get_bir_simp_jgmt_start_label loop_map_ct
-	val wlist = get_bir_simp_jgmt_wlist loop_exit_map_ct
-	val blist = get_bir_simp_jgmt_blist loop_exit_map_ct
+	(* 1. Specialise bir_unsigned_loop_rule_thm *)
+	val prog = get_bir_cont_prog loop_exit_map_ct
+	val start_label = get_bir_cont_start_label loop_map_ct
+	val ilist = get_bir_cont_ilist loop_exit_map_ct
+	val elist = get_bir_cont_elist loop_exit_map_ct
 
 	val bir_add_comp_while_rule_thm =
 	  ISPECL [prog,
 		  start_label,
-		  wlist,
-		  blist,
+		  ilist,
+		  elist,
 		  loop_invariant,
 		  loop_condition,
 		  loop_variant,
-		  get_bir_simp_jgmt_post loop_exit_map_ct]
-                 bir_wm_instTheory.bir_simp_unsigned_loop_rule_thm
+		  get_bir_cont_post loop_exit_map_ct]
+                 bir_tsTheory.bir_unsigned_loop_rule_thm
 
 	(* 2. Knock out antecedents:  *)
 	(* Note: This structure enforces the property that each step only touches the
@@ -595,20 +595,20 @@ open bir_inst_liftingHelpersLib;
 						     bir_add_reg_prog_def needed *)
 				     )] bir_add_comp_while_rule_thm3
 
-	(* Start label should not be in whitelist *)
+	(* Start label should not be in include list *)
 	val bir_add_comp_while_rule_thm5 =
 	  SIMP_RULE std_ss [prove((fst o dest_imp o concl) bir_add_comp_while_rule_thm4,
 				       simp_in_set_repr_tac
 				     )] bir_add_comp_while_rule_thm4
 
-	(* Start label should not be in blacklist *)
+	(* Start label should not be in exclude list *)
 	(* TODO: Construct this antecedent explicitly in place *)
 	val bir_add_comp_while_rule_thm6 =
 	  SIMP_RULE std_ss [prove((fst o dest_imp o concl) bir_add_comp_while_rule_thm5,
 				       simp_in_set_repr_tac
 				     )] bir_add_comp_while_rule_thm5
 
-	(* Intersection of whitelist and blacklist should be empty set *)
+	(* Intersection of include list and exclude list should be empty set *)
 	(* TODO: Construct this antecedent explicitly in place *)
 	val bir_add_comp_while_rule_thm7 =
 	  SIMP_RULE std_ss [prove((fst o dest_imp o concl) bir_add_comp_while_rule_thm6,
@@ -621,11 +621,11 @@ open bir_inst_liftingHelpersLib;
 	    ASSUME_TAC (Q.SPEC `x` (GENL [``v:word64``] loop_map_ct)) >>
 	    FULL_SIMP_TAC (std_ss++inter_set_repr_ss++union_set_repr_ss) [] >>
 	    FULL_SIMP_TAC (std_ss++pred_setLib.PRED_SET_ss) [] >>
-	    FULL_SIMP_TAC std_ss [bir_wm_instTheory.bir_simp_jgmt_def,
-				  abstract_simp_hoare_logicTheory.abstract_simp_jgmt_def,
-				  abstract_hoare_logicTheory.abstract_jgmt_def,
-				  bir_wm_instTheory.bir_exec_to_labels_triple_precond_def,
-				  bir_wm_instTheory.bir_exec_to_labels_triple_postcond_def] >>
+	    FULL_SIMP_TAC std_ss [bir_tsTheory.bir_cont_def,
+				  total_ext_program_logicTheory.t_ext_jgmt_def,
+				  total_program_logicTheory.t_jgmt_def,
+				  bir_tsTheory.bir_exec_to_labels_triple_precond_def,
+				  bir_tsTheory.bir_exec_to_labels_triple_postcond_def] >>
 	    REPEAT STRIP_TAC >> (
               FULL_SIMP_TAC (std_ss++pred_setLib.PRED_SET_ss) []
             ) >>
@@ -671,10 +671,10 @@ open bir_inst_liftingHelpersLib;
               ),
 
               (* bool_exp_env of invariant *)
-	      FULL_SIMP_TAC (std_ss++abstract_hoare_logicSimps.bir_wm_SS)
-		[bir_bool_expTheory.bir_is_bool_exp_env_def, bir_wm_instTheory.bir_etl_wm_def, bir_wm_instTheory.bir_weak_trs_def] >>
+	      FULL_SIMP_TAC (std_ss++program_logicSimps.bir_wm_SS)
+		[bir_bool_expTheory.bir_is_bool_exp_env_def, bir_tsTheory.bir_ts_def, bir_tsTheory.bir_weak_trs_def] >>
               Cases_on `bir_exec_to_labels
-                (^(pred_setSyntax.mk_set [start_label]) UNION (^wlist))
+                (^(pred_setSyntax.mk_set [start_label]) UNION (^ilist))
                 ((^prog):'a bir_program_t) s` >> (
                 FULL_SIMP_TAC (std_ss++HolBACoreSimps.holBACore_ss) [bir_programTheory.bir_exec_to_labels_def]
               ) >>
@@ -701,59 +701,59 @@ open bir_inst_liftingHelpersLib;
       end
     ;
 
-    (* This function composes two bir_simp_jgmts sequentially using bir_simp_std_seq_rule_thm *)
+    (* This function composes two bir_conts sequentially using bir_std_seq_rule_thm *)
     (* TODO: Fix the mess with def_list unfolding too much back and forth,
      *       see if RESTR_EVAL_RULE can be helpful *)
     fun bir_compose_seq_assmpt (get_labels_from_set_repr, simp_in_sing_set_repr_rule,
                                 simp_inter_set_repr_rule)
-          simp_ct1 simp_ct2 def_list assmpt =
+          bir_cont_thm1 bir_cont_thm2 def_list assmpt =
       let
-	(* 1. Specialise bir_simp_std_seq_rule_thm *)
-	val prog = get_bir_simp_jgmt_prog simp_ct1
-        val invariant = get_bir_simp_jgmt_invariant simp_ct1
-	val white_ending_label_set1 = get_bir_simp_jgmt_wlist simp_ct1
-	val white_ending_label_set2 = get_bir_simp_jgmt_wlist simp_ct2
-	val black_ending_label_set1 = get_bir_simp_jgmt_blist simp_ct1
-	val black_ending_label_set2 = get_bir_simp_jgmt_blist simp_ct2
-	val start_label = get_bir_simp_jgmt_start_label simp_ct1
-	val pre1 = get_bir_simp_jgmt_pre simp_ct1
-	val post1 = get_bir_simp_jgmt_post simp_ct1
-	val post2 = get_bir_simp_jgmt_post simp_ct2
+	(* 1. Specialise bir_std_seq_rule_thm *)
+	val prog = get_bir_cont_prog bir_cont_thm1
+        val invariant = get_bir_cont_invariant bir_cont_thm1
+	val include_ending_label_set1 = get_bir_cont_ilist bir_cont_thm1
+	val include_ending_label_set2 = get_bir_cont_ilist bir_cont_thm2
+	val exclude_ending_label_set1 = get_bir_cont_elist bir_cont_thm1
+	val exclude_ending_label_set2 = get_bir_cont_elist bir_cont_thm2
+	val start_label = get_bir_cont_start_label bir_cont_thm1
+	val pre1 = get_bir_cont_pre bir_cont_thm1
+	val post1 = get_bir_cont_post bir_cont_thm1
+	val post2 = get_bir_cont_post bir_cont_thm2
 
-        (* TODO: HO_MATCH_MP is not general enough to immediately knock out the bir_simp_jgmt
+        (* TODO: HO_MATCH_MP is not general enough to immediately knock out the bir_cont
          * antecedent before specialisation *)
 	val bir_add_comp_seq_rule_thm =
-	  ISPECL [prog, white_ending_label_set1, white_ending_label_set2,
-		  black_ending_label_set1, black_ending_label_set2,
+	  ISPECL [prog, include_ending_label_set1, include_ending_label_set2,
+		  exclude_ending_label_set1, exclude_ending_label_set2,
 		  invariant, start_label, pre1, post1, post2]
-	    bir_wm_instTheory.bir_simp_std_seq_rule_thm
+	    bir_tsTheory.bir_std_seq_rule_thm
 
 	(* 2. Knock out antecedents: *)
-	(* Whitelist of contract 2 should be subset of blacklist of contract 1 *)
+	(* Include list of contract 2 should be subset of exclude list of contract 1 *)
 	val bir_add_comp_seq_rule_thm1 =
 	  SIMP_RULE std_ss [prove (pred_setSyntax.mk_subset
-                                     (white_ending_label_set2,
-                                      black_ending_label_set1),
+                                     (include_ending_label_set2,
+                                      exclude_ending_label_set1),
 
 				       SIMP_TAC (std_ss++pred_setLib.PRED_SET_ss)
                                          [pred_setTheory.SUBSET_DEF]
                             )] bir_add_comp_seq_rule_thm
 
-	(* The intersection between whitelist of contract 1 and whitelist of contract 2 should be empty *)
+	(* The intersection between include list of contract 1 and include list of contract 2 should be empty *)
         (* TODO: Does this work for larger than singleton sets? *)
 	val spec_noteq_trans_impl1 =
-	  ISPECL [el 1 (get_labels_from_set_repr white_ending_label_set1),
-		  el 1 (get_labels_from_set_repr white_ending_label_set2)]
+	  ISPECL [el 1 (get_labels_from_set_repr include_ending_label_set1),
+		  el 1 (get_labels_from_set_repr include_ending_label_set2)]
             bir_auxiliaryTheory.noteq_trans_impl
-        val white_inter_lbls = (get_labels_from_set_repr white_ending_label_set1)@
-                               (get_labels_from_set_repr white_ending_label_set2)
-        val cases_on_x_lbls_tac = List.foldr (fn (lbl, st) => Cases_on `x = ^lbl` >> st) ALL_TAC white_inter_lbls
+        val include_inter_lbls = (get_labels_from_set_repr include_ending_label_set1)@
+                               (get_labels_from_set_repr include_ending_label_set2)
+        val cases_on_x_lbls_tac = List.foldr (fn (lbl, st) => Cases_on `x = ^lbl` >> st) ALL_TAC include_inter_lbls
 	val bir_add_comp_seq_rule_thm2 =
 	  SIMP_RULE std_ss [UNDISCH_ALL (prove (mk_imp (assmpt,
                                     mk_eq
                                      (pred_setSyntax.mk_inter
-                                        (white_ending_label_set1,
-                                         white_ending_label_set2),
+                                        (include_ending_label_set1,
+                                         include_ending_label_set2),
                                      pred_setSyntax.mk_empty bir_label_t_ty)),
                             (* TODO: srw_ss()... *)
                             STRIP_TAC >>
@@ -766,18 +766,18 @@ open bir_inst_liftingHelpersLib;
                               )
                             ))] bir_add_comp_seq_rule_thm1
 
-	(* Knock out the bir_simp_jgmt-antecedent *)
+	(* Knock out the bir_cont-antecedent *)
 	val bir_add_comp_seq_rule_thm3 =
-	  HO_MATCH_MP bir_add_comp_seq_rule_thm2 simp_ct1
+	  HO_MATCH_MP bir_add_comp_seq_rule_thm2 bir_cont_thm1
 
-	(* Starting label of contract 2 is the single label in whitelist of contract 1
+	(* Starting label of contract 2 is the single label in include list of contract 1
 	 * Note: The theorem used for composition actually allows for multiple connection points *)
 	val bir_add_comp_seq_rule_thm4 =
           simp_in_sing_set_repr_rule bir_add_comp_seq_rule_thm3
-	(* Knock out the final antecedent with bir_simp_loop_jgmt *)
+	(* Knock out the final antecedent with loop contract *)
 	val bir_add_comp_seq_rule_thm5 =
           HO_MATCH_MP (SIMP_RULE std_ss def_list bir_add_comp_seq_rule_thm4)
-            (SIMP_RULE std_ss def_list simp_ct2)
+            (SIMP_RULE std_ss def_list bir_cont_thm2)
         (* Clean-up the expanded definitions *)
 	val bir_add_comp_seq_rule_thm6 =
           simp_inter_set_repr_rule (SIMP_RULE std_ss (map GSYM def_list) bir_add_comp_seq_rule_thm5)
@@ -791,12 +791,12 @@ open bir_inst_liftingHelpersLib;
 
     fun bir_compose_seq (get_labels_from_set_repr, simp_in_sing_set_repr_rule,
                          simp_inter_set_repr_rule)
-          simp_ct1 simp_ct2 def_list
+          bir_cont_thm1 bir_cont_thm2 def_list
        =
         ((REWRITE_RULE []) o DISCH_ALL) (
           bir_compose_seq_assmpt (get_labels_from_set_repr, simp_in_sing_set_repr_rule,
                                   simp_inter_set_repr_rule)
-            simp_ct1 simp_ct2 def_list T
+            bir_cont_thm1 bir_cont_thm2 def_list T
         )
        ;
 
@@ -865,7 +865,7 @@ open bir_inst_liftingHelpersLib;
       SIMP_RULE std_ss [pred_setTheory.IN_SING]
 
     fun simp_inter_set_rule ct =
-      ONCE_REWRITE_RULE [EVAL (get_bir_simp_jgmt_blist ct)] ct
+      ONCE_REWRITE_RULE [EVAL (get_bir_cont_elist ct)] ct
 
     val simp_in_set_tac =
       SIMP_TAC (std_ss++HolBACoreSimps.holBACore_ss++wordsLib.WORD_ss++pred_setLib.PRED_SET_ss) []
@@ -880,16 +880,16 @@ open bir_inst_liftingHelpersLib;
     *)
 
    (* These are instantiations of composition rules for pred_sets *)
-   val label_ct_to_simp_ct_predset =
-     label_ct_to_simp_ct (not_empty_set, ending_set_to_sml_list, el_in_set, delete_not_empty_set, mk_set,
+   val bir_exec_to_labels_triple_to_bir_cont_predset =
+     bir_exec_to_labels_triple_to_bir_cont (not_empty_set, ending_set_to_sml_list, el_in_set, delete_not_empty_set, mk_set,
 			 simp_delete_set_rule, simp_insert_set_rule);
 
-   val label_ct_to_simp_ct_assmpt_predset =
-     label_ct_to_simp_ct_assmpt (not_empty_set, ending_set_to_sml_list, el_in_set, delete_not_empty_set, mk_set,
+   val bir_exec_to_labels_triple_to_bir_cont_assmpt_predset =
+     bir_exec_to_labels_triple_to_bir_cont_assmpt (not_empty_set, ending_set_to_sml_list, el_in_set, delete_not_empty_set, mk_set,
 			        simp_delete_set_rule, simp_insert_set_rule);
 
-   val label_ct_to_simp_ct_no_taut_assmpt_predset =
-     label_ct_to_simp_ct_no_taut_assmpt (not_empty_set, ending_set_to_sml_list, el_in_set, delete_not_empty_set,
+   val bir_exec_to_labels_triple_to_bir_cont_no_taut_assmpt_predset =
+     bir_exec_to_labels_triple_to_bir_cont_no_taut_assmpt (not_empty_set, ending_set_to_sml_list, el_in_set, delete_not_empty_set,
                                         mk_set, simp_delete_set_rule, simp_insert_set_rule);
 
    val bir_compose_seq_predset =
@@ -901,9 +901,9 @@ open bir_inst_liftingHelpersLib;
      bir_compose_seq_assmpt (ending_set_to_sml_list, simp_in_sing_set_rule,
                              simp_inter_set_rule);
 
-   val bir_remove_labels_from_wlist_predset = bir_remove_labels_from_wlist (not_empty_set);
+   val bir_remove_labels_from_ilist_predset = bir_remove_labels_from_ilist (not_empty_set);
 
-   val bir_remove_labels_from_blist_predset = bir_remove_labels_from_blist (simp_in_set_tac);
+   val bir_remove_labels_from_elist_predset = bir_remove_labels_from_elist (simp_in_set_tac);
 
    val bir_compose_simp_loop_predset =
      bir_compose_simp_loop (simp_in_set_tac, bir_inter_var_set_ss, bir_union_var_set_ss);
@@ -911,8 +911,8 @@ open bir_inst_liftingHelpersLib;
    val bir_compose_simp_loop_unsigned_predset =
      bir_compose_simp_loop_unsigned (simp_in_set_tac, bir_inter_var_set_ss, bir_union_var_set_ss);
 
-   val bir_populate_blacklist_predset =
-     bir_populate_blacklist (ending_set_to_sml_list, el_in_set,
+   val bir_populate_elist_predset =
+     bir_populate_elist (ending_set_to_sml_list, el_in_set,
                                    delete_not_empty_set, mk_set,
                                    simp_delete_set_rule, simp_insert_set_rule);
 
