src/theory/tools/comp/bir_tsScript.sml
@@ -17,22 +17,22 @@ open bir_typing_progTheory;
 open bir_exp_tautologiesTheory;
 open bir_htTheory;
 
-open abstract_hoare_logic_auxTheory;
-open abstract_hoare_logicTheory;
-open abstract_simp_hoare_logicTheory;
+open transition_systemTheory;
+open total_program_logicTheory;
+open total_ext_program_logicTheory;
 
-open abstract_hoare_logicSimps;
+open program_logicSimps;
 open HolBACoreSimps;
 
 open bir_immSyntax;
 
-val _ = new_theory "bir_wm_inst";
+val _ = new_theory "bir_ts";
 
 (******************************************************************)
 (*                         DEFINITIONS                            *)
 (******************************************************************)
 
-(* The transition of the BIR WM *)
+(* The transition of the BIR transition system *)
 val bir_trs_def = Define `
   bir_trs (prog:'a bir_program_t) st =
   let
@@ -44,7 +44,7 @@ val bir_trs_def = Define `
 `;
 
 
-(* The weak transition of the BIR WM *)
+(* The weak transition of the BIR transition system *)
 val bir_weak_trs_def = Define `
   bir_weak_trs ls prog st =
     case (bir_exec_to_labels ls prog st) of
@@ -56,19 +56,16 @@ val bir_weak_trs_def = Define `
 `;
 
 
-(* The BIR WM which is later proven to obey the property
- * "weak_model". *)
-val bir_etl_wm_def =
-  Define `bir_etl_wm (prog :'a bir_program_t) = <|
+(* The BIR transition system which is later proven to obey the property
+ * "first_enc". *)
+val bir_ts_def =
+  Define `bir_ts (prog :'a bir_program_t) = <|
     trs  := bir_trs prog;
-    weak := (\st ls st'.
+    weak := (\ls st st'.
 	       (bir_weak_trs ls prog st = SOME st')
 	    );
-    pc   := (\st. st.bst_pc.bpc_label)
+    ctrl   := (\st. st.bst_pc.bpc_label)
   |>`;
-
-(* bir_exec_to_labels_triple_def *)
-(* abstract_jgmt_def *)
 
 val bir_exec_to_labels_triple_precond_def = Define `
   bir_exec_to_labels_triple_precond st pre prog =
@@ -81,7 +78,7 @@ val bir_exec_to_labels_triple_precond_def = Define `
 `;
 
 (* We don't need the condition that st.bst_pc.bpc_label IN ls here,
- * since we can obtain that result from weak_pc_in_thm. *)
+ * since we can obtain that result from weak_ctrl_in. *)
 val bir_exec_to_labels_triple_postcond_def = Define `
   bir_exec_to_labels_triple_postcond st post prog =
     ((bir_eval_exp (post st.bst_pc.bpc_label) st.bst_environ =
@@ -94,10 +91,10 @@ val bir_exec_to_labels_triple_postcond_def = Define `
 `;
 
 
-(* BIR map triple, mirroring abstract_simp_jgmt *)
-val bir_simp_jgmt_def = Define `
-  bir_simp_jgmt prog invariant (l:bir_label_t) ls ls' pre post =
-    abstract_simp_jgmt (bir_etl_wm prog)
+(* BIR contract, mirroring t_ext_jgmt *)
+val bir_cont_def = Define `
+  bir_cont prog invariant (l:bir_label_t) ls ls' pre post =
+    t_ext_jgmt (bir_ts prog)
       (\s. bir_exec_to_labels_triple_precond s invariant prog)
       l ls ls'
       (\s. bir_exec_to_labels_triple_precond s pre prog)
@@ -299,16 +296,16 @@ EQ_TAC >| [
 
 
 (******************************************************************)
-(*             Proof BIR instantiates weak model                  *)
+(*        Proof BIR transition system is first-encounter          *)
 (******************************************************************)
 
-val bir_model_is_weak = store_thm("bir_model_is_weak",
+val bir_ts_first_enc = store_thm("bir_ts_first_enc",
   ``!(prog: 'a bir_program_t).
-      weak_model (bir_etl_wm prog)``,
+      first_enc (bir_ts prog)``,
 
 REPEAT STRIP_TAC >>
 FULL_SIMP_TAC (std_ss++bir_wm_SS)
-              [weak_model_def, bir_etl_wm_def] >>
+              [first_enc_def, bir_ts_def] >>
 FULL_SIMP_TAC std_ss [bir_weak_trs_def, LET_DEF] >>
 (* Need to show that bir_exec_to_labels is equivalent to some
  * non-zero application of bir_trs, where label set is touched in
@@ -321,7 +318,7 @@ CASE_TAC >| [
   CASE_TAC >| [
     (* Case 1A: Ended + Final state has status Running - regular
      *          case *)
-    subgoal `?m c_l'. (m > 0) /\ (bir_exec_block_n prog ms m = (l,n,c_l',b))` >- (
+    subgoal `?m c_l'. (m > 0) /\ (bir_exec_block_n prog s m = (l,n,c_l',b))` >- (
       FULL_SIMP_TAC std_ss [bir_exec_to_labels_def] >>
       IMP_RES_TAC bir_exec_to_labels_n_TO_bir_exec_block_n >>
       Q.EXISTS_TAC `m` >>
@@ -386,9 +383,9 @@ CASE_TAC >| [
 	  QSPECL_X_ASSUM
 	    ``!n'.
 	       n' < m' /\ n' > 0 ==>
-	       ?ms''.
-		   (FUNPOW_OPT (bir_trs prog) n' st = SOME ms'') /\
-		   ms''.bst_pc.bpc_label NOTIN ls`` [`m`] >>
+	       ?s''.
+		   (FUNPOW_OPT (bir_trs prog) n' st = SOME s'') /\
+		   s''.bst_pc.bpc_label NOTIN ls`` [`m`] >>
 	  REV_FULL_SIMP_TAC arith_ss [] >>
 	  IMP_RES_TAC bir_exec_block_n_to_FUNPOW_OPT_bir_trs >>
 	  REV_FULL_SIMP_TAC (std_ss++holBACore_ss) [] >>
@@ -422,7 +419,7 @@ CASE_TAC >| [
      * value of FUNPOW_OPT (bir_trs prog) would be NONE). *)
     FULL_SIMP_TAC std_ss [GSYM boolTheory.IMP_DISJ_THM] >>
     REPEAT STRIP_TAC >>
-    rename1 `FUNPOW_OPT (bir_trs prog) n' st = SOME ms'` >>
+    rename1 `FUNPOW_OPT (bir_trs prog) n' st = SOME s'` >>
     rename1 `FUNPOW_OPT (bir_trs prog) n' st = SOME st''` >>
     rename1
       `bir_exec_to_labels ls prog st = BER_Ended l n n0 st'` >>
@@ -480,7 +477,7 @@ CASE_TAC >| [
   rename1 `m > 0` >>
   REPEAT STRIP_TAC >>
   IMP_RES_TAC FUNPOW_OPT_bir_trs_to_bir_exec_block_n >>
-  rename1 `bir_exec_block_n prog st m = (l',n,c_l',ms')` >>
+  rename1 `bir_exec_block_n prog st m = (l',n,c_l',s')` >>
   rename1 `bir_exec_block_n prog st m = (l',n,c_l',st')` >>
   (* Then, bir_exec_to_labels_looping_not_reached_ls gives us
    * contradiction on label set membership *)
@@ -493,17 +490,17 @@ CASE_TAC >| [
 (* BIR map triple theorems                           *)
 (*****************************************************)
 
-(* Obtaining a bir_simp_jgmt from a bir_exec_to_labels_triple *)
+(* Obtaining a bir_cont from a bir_exec_to_labels_triple *)
 val bir_label_jgmt_impl_weak_jgmt =
   store_thm("bir_label_jgmt_impl_weak_jgmt",
   ``!prog l ls pre post.
     ls <> {} ==>
     bir_exec_to_labels_triple prog l ls pre post ==>
-    bir_simp_jgmt prog bir_exp_true l ls {} pre post``,
+    bir_cont prog bir_exp_true l ls {} pre post``,
 
 FULL_SIMP_TAC (std_ss++bir_wm_SS)
-              [bir_simp_jgmt_def, abstract_simp_jgmt_def,
-               abstract_jgmt_def, bir_etl_wm_def,
+              [bir_cont_def, t_ext_jgmt_def,
+               t_jgmt_def, bir_ts_def,
                bir_exec_to_labels_triple_def,
                bir_exec_to_labels_triple_precond_def,
                bir_exec_to_labels_triple_postcond_def] >>
@@ -521,68 +518,68 @@ ASM_SIMP_TAC std_ss [bir_eval_exp_TF, bir_is_bool_exp_env_REWRS]
 );
 
 (* This theorem moves ending labels which are implicitly
- * blacklisted by the postcondition from the whitelist of a bir_simp_jgmt to the blacklist. *)
-val bir_simp_wl_to_bl_rule_thm = store_thm("bir_simp_wl_to_bl_rule_thm",
-  ``!prog inv l wlist blist pre post elabel.
-    bir_simp_jgmt prog inv l wlist blist pre post ==>
-    elabel IN wlist ==>
-    wlist DELETE elabel <> {} ==>
+ * excluded by the postcondition from the include list of a bir_cont to the exclude list. *)
+val bir_il_to_el_rule_thm = store_thm("bir_il_to_el_rule_thm",
+  ``!prog inv l ilist elist pre post elabel.
+    bir_cont prog inv l ilist elist pre post ==>
+    elabel IN ilist ==>
+    ilist DELETE elabel <> {} ==>
     (post elabel = bir_exp_false) ==>
-    bir_simp_jgmt prog inv l (wlist DELETE elabel) (elabel INSERT blist) pre post``,
+    bir_cont prog inv l (ilist DELETE elabel) (elabel INSERT elist) pre post``,
 
 REPEAT STRIP_TAC >>
-FULL_SIMP_TAC std_ss [bir_simp_jgmt_def] >>
-irule abstract_simp_wl_to_bl_rule_thm >>
-ASSUME_TAC bir_model_is_weak >>
+FULL_SIMP_TAC std_ss [bir_cont_def] >>
+irule total_ext_il_to_el_rule_thm >>
+ASSUME_TAC bir_ts_first_enc >>
 QSPECL_X_ASSUM ``!prog. _`` [`prog`] >>
 FULL_SIMP_TAC std_ss [] >>
 GEN_TAC >> DISCH_TAC >>
 SIMP_TAC std_ss [bir_exec_to_labels_triple_postcond_def] >>
-FULL_SIMP_TAC (std_ss++bir_wm_SS) [bir_etl_wm_def, bir_eval_exp_TF, bir_val_TF_dist]
+FULL_SIMP_TAC (std_ss++bir_wm_SS) [bir_ts_def, bir_eval_exp_TF, bir_val_TF_dist]
 );
 
-val bir_simp_wl_to_bl_set_rule_thm = store_thm("bir_simp_wl_to_bl_set_rule_thm",
-  ``!prog inv l wlist blist pre post elabels.
-    bir_simp_jgmt prog inv l wlist blist pre post ==>
+val bir_il_to_el_set_rule_thm = store_thm("bir_il_to_el_set_rule_thm",
+  ``!prog inv l ilist elist pre post elabels.
+    bir_cont prog inv l ilist elist pre post ==>
     FINITE elabels ==>
-    elabels PSUBSET wlist ==>
+    elabels PSUBSET ilist ==>
     (!elabel. elabel IN elabels ==> (post elabel = bir_exp_false)) ==>
-    bir_simp_jgmt prog inv l (wlist DIFF elabels) (elabels UNION blist) pre post``,
+    bir_cont prog inv l (ilist DIFF elabels) (elabels UNION elist) pre post``,
 
 REPEAT STRIP_TAC >>
-FULL_SIMP_TAC std_ss [bir_simp_jgmt_def, pred_setTheory.UNION_COMM] >>
-irule abstract_simp_wl_to_bl_set_rule_thm >>
-ASSUME_TAC bir_model_is_weak >>
+FULL_SIMP_TAC std_ss [bir_cont_def, Once pred_setTheory.UNION_COMM] >>
+irule total_ext_il_to_el_set_rule_thm >>
+ASSUME_TAC bir_ts_first_enc >>
 QSPECL_X_ASSUM ``!prog. _`` [`prog`] >>
 FULL_SIMP_TAC std_ss [] >>
 NTAC 2 STRIP_TAC >>
-QSPECL_X_ASSUM ``!prog. _`` [`(bir_etl_wm prog).pc ms`] >>
+QSPECL_X_ASSUM ``!prog. _`` [`(bir_ts prog).ctrl s`] >>
 SIMP_TAC std_ss [bir_exec_to_labels_triple_postcond_def] >>
-FULL_SIMP_TAC (std_ss++bir_wm_SS) [bir_etl_wm_def, bir_eval_exp_TF, bir_val_TF_dist]
+FULL_SIMP_TAC (std_ss++bir_wm_SS) [bir_ts_def, bir_eval_exp_TF, bir_val_TF_dist]
 );
 
 
-val bir_simp_post_weak_rule_thm = store_thm("bir_simp_post_weak_rule_thm",
+val bir_post_weak_rule_thm = store_thm("bir_post_weak_rule_thm",
   ``!prog invariant l ls ls' pre post1 post2.
     (!st.
      st.bst_pc.bpc_label IN ls ==>
      (bir_eval_exp (post1 st.bst_pc.bpc_label) st.bst_environ = SOME bir_val_true) ==>
      (bir_eval_exp (post2 st.bst_pc.bpc_label) st.bst_environ = SOME bir_val_true)
     ) ==>
-    bir_simp_jgmt prog invariant l ls ls' pre post1 ==>
-    bir_simp_jgmt prog invariant l ls ls' pre post2``,
+    bir_cont prog invariant l ls ls' pre post1 ==>
+    bir_cont prog invariant l ls ls' pre post2``,
 
 REPEAT STRIP_TAC >>
-FULL_SIMP_TAC std_ss [bir_simp_jgmt_def] >>
-irule abstract_simp_post_weak_rule_thm >>
+FULL_SIMP_TAC std_ss [bir_cont_def] >>
+irule total_ext_post_weak_rule_thm >>
 REPEAT STRIP_TAC >- (
-  METIS_TAC [bir_model_is_weak]
+  METIS_TAC [bir_ts_first_enc]
 ) >>
 Q.EXISTS_TAC `\s'. bir_exec_to_labels_triple_postcond s' post1 prog` >>
 REPEAT STRIP_TAC >| [
-  QSPECL_X_ASSUM ``!st. _`` [`ms`] >>
-  Q.SUBGOAL_THEN `ms.bst_pc.bpc_label IN ls` (fn thm => FULL_SIMP_TAC std_ss [thm]) >- (
-    FULL_SIMP_TAC (std_ss++bir_wm_SS) [bir_etl_wm_def]
+  QSPECL_X_ASSUM ``!st. _`` [`s`] >>
+  Q.SUBGOAL_THEN `s.bst_pc.bpc_label IN ls` (fn thm => FULL_SIMP_TAC std_ss [thm]) >- (
+    FULL_SIMP_TAC (std_ss++bir_wm_SS) [bir_ts_def]
   ) >>
   FULL_SIMP_TAC std_ss [bir_exec_to_labels_triple_postcond_def, bir_is_bool_exp_env_def,
                         bir_val_true_def] >>
@@ -593,17 +590,17 @@ REPEAT STRIP_TAC >| [
 );
 
 
-val bir_simp_taut_pre_str_rule_thm = store_thm("bir_simp_taut_pre_str_rule_thm",
+val bir_taut_pre_str_rule_thm = store_thm("bir_taut_pre_str_rule_thm",
   ``!prog invariant l ls ls' pre1 pre2 post.
     ((bir_vars_of_exp pre2) SUBSET (bir_vars_of_program prog)) ==>
     ((bir_vars_of_exp pre1) SUBSET (bir_vars_of_program prog)) ==>
     bir_exp_is_taut
       (BExp_BinExp BIExp_Or (BExp_UnaryExp BIExp_Not pre2) pre1) ==>
-    bir_simp_jgmt prog invariant l ls ls' pre1 post ==>
-    bir_simp_jgmt prog invariant l ls ls' pre2 post``,
+    bir_cont prog invariant l ls ls' pre1 post ==>
+    bir_cont prog invariant l ls ls' pre2 post``,
 
 REPEAT STRIP_TAC >>
-FULL_SIMP_TAC std_ss [bir_simp_jgmt_def, abstract_simp_jgmt_def, abstract_jgmt_def,
+FULL_SIMP_TAC std_ss [bir_cont_def, t_ext_jgmt_def, t_jgmt_def,
                       bir_exec_to_labels_triple_precond_def] >>
 REPEAT STRIP_TAC >>
 PAT_X_ASSUM ``!s. _`` (fn thm => ASSUME_TAC (Q.SPEC `s` thm)) >>
@@ -636,17 +633,17 @@ METIS_TAC []
 );
 
 
-val bir_simp_taut_post_weak_rule_thm = store_thm("bir_simp_taut_post_weak_rule_thm",
+val bir_taut_post_weak_rule_thm = store_thm("bir_taut_post_weak_rule_thm",
   ``!prog invariant l ls l2 ls' pre post1 post2.
     ((bir_vars_of_exp (post1 l2)) SUBSET (bir_vars_of_program prog)) ==>
     ((bir_vars_of_exp (post2 l2)) SUBSET (bir_vars_of_program prog)) ==>
     (!l'. (l' <> l2) ==> (post1 l' = post2 l')) ==>
     bir_exp_is_taut
       (BExp_BinExp BIExp_Or (BExp_UnaryExp BIExp_Not (post1 l2)) (post2 l2)) ==>
-    bir_simp_jgmt prog invariant l ls ls' pre post1 ==>
-    bir_simp_jgmt prog invariant l ls ls' pre post2``,
+    bir_cont prog invariant l ls ls' pre post1 ==>
+    bir_cont prog invariant l ls ls' pre post2``,
 
-FULL_SIMP_TAC std_ss [bir_simp_jgmt_def, abstract_simp_jgmt_def, abstract_jgmt_def,
+FULL_SIMP_TAC std_ss [bir_cont_def, t_ext_jgmt_def, t_jgmt_def,
                       bir_exec_to_labels_triple_postcond_def] >>
 REPEAT STRIP_TAC >>
 PAT_X_ASSUM ``!s. _`` (fn thm => ASSUME_TAC (Q.SPEC `s` thm)) >>
@@ -679,37 +676,37 @@ METIS_TAC [bir_exp_equivTheory.bir_impl_equiv, bir_exp_tautologiesTheory.bir_exp
 );
 
 
-val bir_simp_std_seq_rule_thm =
-  store_thm("bir_simp_std_seq_rule_thm",
+val bir_std_seq_rule_thm =
+  store_thm("bir_std_seq_rule_thm",
   ``!prog ls1 ls1' ls2 ls2' invariant l pre1 post1 post2.
     ls1' SUBSET ls2 ==>
     (ls1 INTER ls1' = EMPTY) ==>
-    bir_simp_jgmt prog invariant l ls1 ls2 pre1 post1 ==>
-    (!l1. (l1 IN ls1) ==> (bir_simp_jgmt prog invariant l1 ls1' ls2' (post1 l1) post2)) ==>
-    bir_simp_jgmt prog invariant l ls1' (ls2 INTER ls2') pre1 post2``,
+    bir_cont prog invariant l ls1 ls2 pre1 post1 ==>
+    (!l1. (l1 IN ls1) ==> (bir_cont prog invariant l1 ls1' ls2' (post1 l1) post2)) ==>
+    bir_cont prog invariant l ls1' (ls2 INTER ls2') pre1 post2``,
 
 REPEAT STRIP_TAC >>
-FULL_SIMP_TAC std_ss [bir_simp_jgmt_def] >>
-irule abstract_simp_std_seq_rule_thm >>
+FULL_SIMP_TAC std_ss [bir_cont_def] >>
+irule total_ext_std_seq_rule_thm >>
 REPEAT STRIP_TAC >- (
-  METIS_TAC [bir_model_is_weak]
+  METIS_TAC [bir_ts_first_enc]
 ) >> (
   FULL_SIMP_TAC std_ss []
 ) >>
 Q.EXISTS_TAC `ls1` >>
-Q.EXISTS_TAC `\s. bir_exec_to_labels_triple_precond s (post1 ((bir_etl_wm prog).pc s)) prog` >>
+Q.EXISTS_TAC `\s. bir_exec_to_labels_triple_precond s (post1 ((bir_ts prog).ctrl s)) prog` >>
 REPEAT STRIP_TAC >> (
   FULL_SIMP_TAC std_ss []
 ) >| [
   QSPECL_X_ASSUM ``!l1. _`` [`l1`] >>
   REV_FULL_SIMP_TAC std_ss [] >>
-  FULL_SIMP_TAC std_ss [abstract_simp_jgmt_def, abstract_jgmt_def,
+  FULL_SIMP_TAC std_ss [t_ext_jgmt_def, t_jgmt_def,
                         bir_exec_to_labels_triple_precond_def],
 
-  FULL_SIMP_TAC (std_ss++bir_wm_SS) [abstract_simp_jgmt_def,
+  FULL_SIMP_TAC (std_ss++bir_wm_SS) [t_ext_jgmt_def,
                                      bir_exec_to_labels_triple_precond_def,
                                      bir_exec_to_labels_triple_postcond_def,
-                                     bir_etl_wm_def]
+                                     bir_ts_def]
 ]
 );
 
@@ -718,8 +715,8 @@ val iv2i_def = Define `
     iv2i (BVal_Imm i) = i
 `;
 
-val bir_simp_signed_loop_rule_thm = store_thm("bir_simp_signed_loop_rule_thm",
-  ``!prog l wl bl invariant C1 variant post.
+val bir_signed_loop_rule_thm = store_thm("bir_signed_loop_rule_thm",
+  ``!prog l il el invariant C1 variant post.
     (* Compute in place using proof procedures: *)
     (*   These two needed to use abstract_simp_loop_rule_thm *)
     (type_of_bir_exp variant = SOME (BType_Imm Bit64)) ==>
@@ -728,12 +725,12 @@ val bir_simp_signed_loop_rule_thm = store_thm("bir_simp_signed_loop_rule_thm",
     bir_is_bool_exp C1 ==>
     (bir_vars_of_exp C1) SUBSET (bir_vars_of_program prog) ==>
     (* Extra for abstract_simp_loop_rule_thm *)
-    l NOTIN wl ==>
-    l NOTIN bl ==>
-    (wl INTER bl = {}) ==>
+    l NOTIN il ==>
+    l NOTIN el ==>
+    (il INTER el = {}) ==>
     (* Obtain bir_loop contract through some rule: *)
     (!x.
-     bir_simp_jgmt prog invariant l ({l} UNION wl) bl
+     bir_cont prog invariant l ({l} UNION il) el
        (BExp_BinExp BIExp_And C1
 	  (BExp_BinPred BIExp_Equal variant (BExp_Const (Imm64 x)))
        )
@@ -746,29 +743,29 @@ val bir_simp_signed_loop_rule_thm = store_thm("bir_simp_signed_loop_rule_thm",
 		    (BExp_Const (Imm64 0w)) variant))
 	    else bir_exp_false)
     ) ==>
-    bir_simp_jgmt prog bir_exp_true l wl bl
+    bir_cont prog bir_exp_true l il el
       (BExp_BinExp BIExp_And invariant (BExp_UnaryExp BIExp_Not C1)) post ==>
-    bir_simp_jgmt prog bir_exp_true l wl bl
+    bir_cont prog bir_exp_true l il el
       invariant
       post``,
 
-FULL_SIMP_TAC std_ss [bir_simp_jgmt_def] >>
+FULL_SIMP_TAC std_ss [bir_cont_def] >>
 REPEAT STRIP_TAC >>
-ASSUME_TAC bir_model_is_weak >>
+ASSUME_TAC bir_ts_first_enc >>
 QSPECL_X_ASSUM ``!prog. _`` [`prog`] >>
 (* 1. Use abstract_simp_loop_rule_thm *)
-Q.SUBGOAL_THEN `abstract_simp_jgmt (bir_etl_wm prog)
-     (\s. bir_exec_to_labels_triple_precond s bir_exp_true prog) l wl bl
+Q.SUBGOAL_THEN `t_ext_jgmt (bir_ts prog)
+     (\s. bir_exec_to_labels_triple_precond s bir_exp_true prog) l il el
      (\s. bir_exec_to_labels_triple_precond s invariant prog)
      (\s'. bir_exec_to_labels_triple_postcond s' post prog) <=>
-  abstract_simp_jgmt (bir_etl_wm prog)
-     (\s. T) l wl bl
+  t_ext_jgmt (bir_ts prog)
+     (\s. T) l il el
      (\s. bir_exec_to_labels_triple_precond s invariant prog)
      (\s'. bir_exec_to_labels_triple_postcond s' post prog)`
   (fn thm => SIMP_TAC std_ss [thm]) >- (
   SIMP_TAC std_ss [bir_exec_to_labels_triple_precond_def] >>
-  FULL_SIMP_TAC std_ss [abstract_simp_jgmt_def] >>
-  SIMP_TAC std_ss [abstract_jgmt_def] >>
+  FULL_SIMP_TAC std_ss [t_ext_jgmt_def] >>
+  SIMP_TAC std_ss [t_jgmt_def] >>
   EQ_TAC >> (
     REPEAT STRIP_TAC >>
     QSPECL_X_ASSUM ``!s. _`` [`s`] >>
@@ -777,16 +774,16 @@ Q.SUBGOAL_THEN `abstract_simp_jgmt (bir_etl_wm prog)
     FULL_SIMP_TAC std_ss [bir_exec_to_labels_triple_postcond_def]
   )
 ) >>
-irule abstract_simp_loop_rule_thm >>
+irule total_ext_loop_rule_thm >>
 FULL_SIMP_TAC std_ss [] >>
 Q.EXISTS_TAC `\s. bir_eval_exp C1 s.bst_environ = SOME bir_val_true` >>
 Q.EXISTS_TAC `\s. b2n (iv2i (THE (bir_eval_exp variant s.bst_environ)))` >>
 STRIP_TAC >| [
   GEN_TAC >>
-  FULL_SIMP_TAC std_ss [abstract_simp_jgmt_def] >>
+  FULL_SIMP_TAC std_ss [t_ext_jgmt_def] >>
   (* Remove unnecessary assumption *)
-  Q.PAT_X_ASSUM `abstract_jgmt a b c d e` (fn thm => ALL_TAC) >>
-  FULL_SIMP_TAC std_ss [abstract_jgmt_def] >>
+  Q.PAT_X_ASSUM `t_jgmt a b c d e` (fn thm => ALL_TAC) >>
+  FULL_SIMP_TAC std_ss [t_jgmt_def] >>
   SIMP_TAC std_ss [bir_exec_to_labels_triple_precond_def] >>
   REPEAT STRIP_TAC >>
   QSPECL_X_ASSUM ``!x. _`` [`n2w x`] >>
@@ -831,7 +828,7 @@ STRIP_TAC >| [
   ) >>
   FULL_SIMP_TAC (std_ss++bir_wm_SS)
     [bir_is_bool_exp_env_REWRS,
-     bir_etl_wm_def, bir_weak_trs_EQ, GSYM bir_and_equiv] >>
+     bir_ts_def, bir_weak_trs_EQ, GSYM bir_and_equiv] >>
   subgoal `b2n (iv2i (THE (bir_eval_exp variant s'.bst_environ))) < x` >- (
     subgoal `?x'. bir_eval_exp variant s'.bst_environ =
 		    SOME (BVal_Imm (Imm64 x'))` >- (
@@ -854,11 +851,11 @@ STRIP_TAC >| [
 
   (* Remove unnecessary assumption *)
   Q.PAT_X_ASSUM `!x. _` (fn thm => ALL_TAC) >>
-  FULL_SIMP_TAC std_ss [abstract_simp_jgmt_def, abstract_jgmt_def] >>
+  FULL_SIMP_TAC std_ss [t_ext_jgmt_def, t_jgmt_def] >>
   REPEAT STRIP_TAC >>
-  QSPECL_X_ASSUM ``!s. _`` [`ms`] >>
+  QSPECL_X_ASSUM ``!s. _`` [`s`] >>
   REV_FULL_SIMP_TAC std_ss [bir_exec_to_labels_triple_precond_def, GSYM bir_and_equiv] >>
-  subgoal `bir_is_bool_exp_env ms.bst_environ C1` >- (
+  subgoal `bir_is_bool_exp_env s.bst_environ C1` >- (
     FULL_SIMP_TAC std_ss [bir_is_bool_exp_env_def] >>
     IMP_RES_TAC bir_env_oldTheory.bir_env_vars_are_initialised_SUBSET
   ) >>
@@ -871,8 +868,8 @@ STRIP_TAC >| [
 );
 
 
-val bir_simp_unsigned_loop_rule_thm = store_thm("bir_simp_unsigned_loop_rule_thm",
-  ``!prog l wl bl invariant C1 variant post.
+val bir_unsigned_loop_rule_thm = store_thm("bir_unsigned_loop_rule_thm",
+  ``!prog l il el invariant C1 variant post.
     (* Compute in place using proof procedures: *)
     (*   These two needed to use abstract_simp_loop_rule_thm *)
     (type_of_bir_exp variant = SOME (BType_Imm Bit64)) ==>
@@ -881,12 +878,12 @@ val bir_simp_unsigned_loop_rule_thm = store_thm("bir_simp_unsigned_loop_rule_thm
     bir_is_bool_exp C1 ==>
     (bir_vars_of_exp C1) SUBSET (bir_vars_of_program prog) ==>
     (* Extra for abstract_simp_loop_rule_thm *)
-    l NOTIN wl ==>
-    l NOTIN bl ==>
-    (wl INTER bl = {}) ==>
+    l NOTIN il ==>
+    l NOTIN el ==>
+    (il INTER el = {}) ==>
     (* Obtain bir_loop contract through some rule: *)
     (!x.
-     bir_simp_jgmt prog invariant l ({l} UNION wl) bl
+     bir_cont prog invariant l ({l} UNION il) el
        (BExp_BinExp BIExp_And C1
 	  (BExp_BinPred BIExp_Equal variant (BExp_Const (Imm64 x)))
        )
@@ -899,30 +896,29 @@ val bir_simp_unsigned_loop_rule_thm = store_thm("bir_simp_unsigned_loop_rule_thm
 		    (BExp_Const (Imm64 0w)) variant))
 	    else bir_exp_false)
     ) ==>
-    bir_simp_jgmt prog bir_exp_true l wl bl
+    bir_cont prog bir_exp_true l il el
       (BExp_BinExp BIExp_And invariant (BExp_UnaryExp BIExp_Not C1)) post ==>
-    bir_simp_jgmt prog bir_exp_true l wl bl
+    bir_cont prog bir_exp_true l il el
       invariant
       post``,
 
-
-FULL_SIMP_TAC std_ss [bir_simp_jgmt_def] >>
+FULL_SIMP_TAC std_ss [bir_cont_def] >>
 REPEAT STRIP_TAC >>
-ASSUME_TAC bir_model_is_weak >>
+ASSUME_TAC bir_ts_first_enc >>
 QSPECL_X_ASSUM ``!prog. _`` [`prog`] >>
 (* 1. Use abstract_simp_loop_rule_thm *)
-Q.SUBGOAL_THEN `abstract_simp_jgmt (bir_etl_wm prog)
-     (\s. bir_exec_to_labels_triple_precond s bir_exp_true prog) l wl bl
+Q.SUBGOAL_THEN `t_ext_jgmt (bir_ts prog)
+     (\s. bir_exec_to_labels_triple_precond s bir_exp_true prog) l il el
      (\s. bir_exec_to_labels_triple_precond s invariant prog)
      (\s'. bir_exec_to_labels_triple_postcond s' post prog) <=>
-  abstract_simp_jgmt (bir_etl_wm prog)
-     (\s. T) l wl bl
+  t_ext_jgmt (bir_ts prog)
+     (\s. T) l il el
      (\s. bir_exec_to_labels_triple_precond s invariant prog)
      (\s'. bir_exec_to_labels_triple_postcond s' post prog)`
   (fn thm => SIMP_TAC std_ss [thm]) >- (
   SIMP_TAC std_ss [bir_exec_to_labels_triple_precond_def] >>
-  FULL_SIMP_TAC std_ss [abstract_simp_jgmt_def] >>
-  SIMP_TAC std_ss [abstract_jgmt_def] >>
+  FULL_SIMP_TAC std_ss [t_ext_jgmt_def] >>
+  SIMP_TAC std_ss [t_jgmt_def] >>
   EQ_TAC >> (
     REPEAT STRIP_TAC >>
     QSPECL_X_ASSUM ``!s. _`` [`s`] >>
@@ -931,16 +927,16 @@ Q.SUBGOAL_THEN `abstract_simp_jgmt (bir_etl_wm prog)
     FULL_SIMP_TAC std_ss [bir_exec_to_labels_triple_postcond_def]
   )
 ) >>
-irule abstract_simp_loop_rule_thm >>
+irule total_ext_loop_rule_thm >>
 FULL_SIMP_TAC std_ss [] >>
 Q.EXISTS_TAC `\s. bir_eval_exp C1 s.bst_environ = SOME bir_val_true` >>
 Q.EXISTS_TAC `\s. b2n (iv2i (THE (bir_eval_exp variant s.bst_environ)))` >>
 STRIP_TAC >| [
   GEN_TAC >>
-  FULL_SIMP_TAC std_ss [abstract_simp_jgmt_def] >>
+  FULL_SIMP_TAC std_ss [t_ext_jgmt_def] >>
   (* Remove unnecessary assumption *)
-  Q.PAT_X_ASSUM `abstract_jgmt a b c d e` (fn thm => ALL_TAC) >>
-  FULL_SIMP_TAC std_ss [abstract_jgmt_def] >>
+  Q.PAT_X_ASSUM `t_jgmt a b c d e` (fn thm => ALL_TAC) >>
+  FULL_SIMP_TAC std_ss [t_jgmt_def] >>
   SIMP_TAC std_ss [bir_exec_to_labels_triple_precond_def] >>
   REPEAT STRIP_TAC >>
   QSPECL_X_ASSUM ``!x. _`` [`n2w x`] >>
@@ -985,7 +981,7 @@ STRIP_TAC >| [
   ) >>
   FULL_SIMP_TAC (std_ss++bir_wm_SS)
     [bir_is_bool_exp_env_REWRS,
-     bir_etl_wm_def, bir_weak_trs_EQ, GSYM bir_and_equiv] >>
+     bir_ts_def, bir_weak_trs_EQ, GSYM bir_and_equiv] >>
   subgoal `b2n (iv2i (THE (bir_eval_exp variant s'.bst_environ))) < x` >- (
     subgoal `?x'. bir_eval_exp variant s'.bst_environ =
 		    SOME (BVal_Imm (Imm64 x'))` >- (
@@ -1006,11 +1002,11 @@ STRIP_TAC >| [
 
   (* Remove unnecessary assumption *)
   Q.PAT_X_ASSUM `!x. _` (fn thm => ALL_TAC) >>
-  FULL_SIMP_TAC std_ss [abstract_simp_jgmt_def, abstract_jgmt_def] >>
+  FULL_SIMP_TAC std_ss [t_ext_jgmt_def, t_jgmt_def] >>
   REPEAT STRIP_TAC >>
-  QSPECL_X_ASSUM ``!s. _`` [`ms`] >>
+  QSPECL_X_ASSUM ``!s. _`` [`s`] >>
   REV_FULL_SIMP_TAC std_ss [bir_exec_to_labels_triple_precond_def, GSYM bir_and_equiv] >>
-  subgoal `bir_is_bool_exp_env ms.bst_environ C1` >- (
+  subgoal `bir_is_bool_exp_env s.bst_environ C1` >- (
     FULL_SIMP_TAC std_ss [bir_is_bool_exp_env_def] >>
     IMP_RES_TAC bir_env_oldTheory.bir_env_vars_are_initialised_SUBSET
   ) >>
@@ -1022,46 +1018,46 @@ STRIP_TAC >| [
 ]
 );
 
-(* Shrinking the whitelist is possible if the corresponding
+(* Shrinking the include list is possible if the corresponding
  * postcondition never holds. *)
-val bir_simp_wl_subset_rule_thm =
- store_thm("bir_simp_wl_subset_rule_thm",
+val bir_il_subset_rule_thm =
+ store_thm("bir_il_subset_rule_thm",
   ``!prog l ls1 ls2 pre post.
     ls1 <> {} ==>
     (!st. (bir_eval_exp (post st.bst_pc.bpc_label) st.bst_environ = SOME bir_val_true) ==>
           (~(st.bst_pc.bpc_label IN ls2))
     ) ==>
-    bir_simp_jgmt prog bir_exp_true l (ls1 UNION ls2) {} pre post ==>
-    bir_simp_jgmt prog bir_exp_true l ls1 {} pre post``,
+    bir_cont prog bir_exp_true l (ls1 UNION ls2) {} pre post ==>
+    bir_cont prog bir_exp_true l ls1 {} pre post``,
 
 REPEAT STRIP_TAC >>
-REV_FULL_SIMP_TAC std_ss [bir_simp_jgmt_def, abstract_simp_jgmt_def,
-                          abstract_jgmt_def] >>
+REV_FULL_SIMP_TAC std_ss [bir_cont_def, t_ext_jgmt_def,
+                          t_jgmt_def] >>
 REPEAT STRIP_TAC >> (
   FULL_SIMP_TAC (std_ss++pred_setLib.PRED_SET_ss) []
 ) >> (
   QSPECL_X_ASSUM ``!s. _`` [`s`] >>
-  ASSUME_TAC (SPECL [``prog:'a bir_program_t``] bir_model_is_weak) >>
+  ASSUME_TAC (SPECL [``prog:'a bir_program_t``] bir_ts_first_enc) >>
   REV_FULL_SIMP_TAC std_ss [] >>
-  IMP_RES_TAC weak_union_pc_not_in_thm >>
+  IMP_RES_TAC weak_union_ctrl_not_in >>
   QSPECL_X_ASSUM ``!st. _`` [`s''`] >>
   subgoal `bir_eval_exp (post s''.bst_pc.bpc_label) s''.bst_environ =
 	    SOME bir_val_true` >- (
     FULL_SIMP_TAC std_ss [bir_exec_to_labels_triple_postcond_def]
   ) >>
-  FULL_SIMP_TAC (std_ss++bir_wm_SS) [bir_etl_wm_def]
+  FULL_SIMP_TAC (std_ss++bir_wm_SS) [bir_ts_def]
 )
 );
 
-val bir_simp_bl_subset_rule_thm =
-  store_thm("bir_simp_bl_subset_rule_thm",
-  ``!prog invariant l wl bl bl' pre post.
-    bl' SUBSET bl ==>
-    bir_simp_jgmt prog invariant l wl bl pre post ==>
-    bir_simp_jgmt prog invariant l wl bl' pre post``,
+val bir_el_subset_rule_thm =
+  store_thm("bir_el_subset_rule_thm",
+  ``!prog invariant l il el el' pre post.
+    el' SUBSET el ==>
+    bir_cont prog invariant l il el pre post ==>
+    bir_cont prog invariant l il el' pre post``,
 
-METIS_TAC [bir_simp_jgmt_def, bir_model_is_weak,
-           abstract_simp_bl_subset_rule_thm]
+METIS_TAC [bir_cont_def, bir_ts_first_enc,
+           total_ext_el_subset_rule_thm]
 );
 
 (* TODO: Move this? *)
@@ -1121,24 +1117,24 @@ Cases_on `bir_get_current_statement prog s.bst_pc` >- (
 FULL_SIMP_TAC std_ss [GSYM bir_get_current_statement_IS_SOME]
 );
 
-val bir_simp_prog_comp_rule_thm =
-  store_thm("bir_simp_prog_comp_rule_thm",
-  ``!prog1 prog2 invariant wl bl l pre post.
+val bir_prog_comp_rule_thm =
+  store_thm("bir_prog_comp_rule_thm",
+  ``!prog1 prog2 invariant il el l pre post.
     bir_is_subprogram prog1 prog2 ==>
     bir_is_valid_labels prog2 ==>
-    bir_simp_jgmt prog1 invariant l wl bl pre post ==>
-    bir_simp_jgmt prog2 invariant l wl bl pre post``,
+    bir_cont prog1 invariant l il el pre post ==>
+    bir_cont prog2 invariant l il el pre post``,
 
 REPEAT STRIP_TAC >>
-FULL_SIMP_TAC std_ss [bir_simp_jgmt_def, abstract_simp_jgmt_def] >>
-FULL_SIMP_TAC (std_ss++bir_wm_SS) [abstract_jgmt_def,
-				   bir_etl_wm_def, bir_weak_trs_def] >>
+FULL_SIMP_TAC std_ss [bir_cont_def, t_ext_jgmt_def] >>
+FULL_SIMP_TAC (std_ss++bir_wm_SS) [t_jgmt_def,
+				   bir_ts_def, bir_weak_trs_def] >>
 REPEAT STRIP_TAC >>
 QSPECL_X_ASSUM ``!s. _`` [`s`] >>
 IMP_RES_TAC bir_exec_to_labels_triple_precond_subprogram >>
 FULL_SIMP_TAC std_ss [] >>
 REV_FULL_SIMP_TAC std_ss [] >>
-Cases_on `bir_exec_to_labels (wl UNION bl) prog1 s` >> (
+Cases_on `bir_exec_to_labels (il UNION el) prog1 s` >> (
   FULL_SIMP_TAC (std_ss++holBACore_ss) []
 ) >>
 Q.PAT_X_ASSUM `b = s'` (fn thm => FULL_SIMP_TAC std_ss [thm]) >>
@@ -1163,26 +1159,26 @@ CONJ_TAC >> (
 )
 );
 
-(* Sketch for alternative proof using abstract_simp_model_comp_rule_thm
+(* Sketch for alternative proof using total_ext_ts_emb_rule_thm
 val bir_map_prog_comp_alt_thm =
   store_thm("bir_map_prog_comp_alt_thm",
-  ``!prog1 prog2 invariant wl bl l pre post.
+  ``!prog1 prog2 invariant il el l pre post.
     bir_is_subprogram prog1 prog2 ==>
     bir_is_valid_labels prog2 ==>
-    bir_simp_jgmt prog1 invariant l wl bl pre post ==>
-    bir_simp_jgmt prog2 invariant l wl bl pre post``,
+    bir_cont prog1 invariant l il el pre post ==>
+    bir_cont prog2 invariant l il el pre post``,
 
 REPEAT STRIP_TAC >>
-FULL_SIMP_TAC std_ss [bir_simp_jgmt_def] >>
-irule abstract_simp_model_comp_rule_thm >>
-FULL_SIMP_TAC std_ss [bir_model_is_weak] >>
-Q.EXISTS_TAC `bir_etl_wm prog1` >>
+FULL_SIMP_TAC std_ss [bir_cont_def] >>
+irule total_ext_ts_emb_rule_thm >>
+FULL_SIMP_TAC std_ss [bir_ts_first_enc] >>
+Q.EXISTS_TAC `bir_ts prog1` >>
 REPEAT STRIP_TAC >| [
-  (* (bir_etl_wm prog1).pc ms = (bir_etl_wm prog2).pc ms *)
-  FULL_SIMP_TAC (std_ss++bir_wm_SS) [bir_etl_wm_def],
+  (* (bir_ts prog1).pc ms = (bir_ts prog2).pc ms *)
+  FULL_SIMP_TAC (std_ss++bir_wm_SS) [bir_ts_def],
 
-  (* (bir_etl_wm prog2).weak ms ls ms' *)
-  FULL_SIMP_TAC (std_ss++bir_wm_SS) [bir_etl_wm_def, bir_weak_trs_def, abstract_simp_jgmt_def] >>
+  (* (bir_ts prog2).weak ms ls ms' *)
+  FULL_SIMP_TAC (std_ss++bir_wm_SS) [bir_ts_def, bir_weak_trs_def, t_ext_jgmt_def] >>
   Cases_on `bir_exec_to_labels ls prog2 ms` >> Cases_on `bir_exec_to_labels ls prog1 ms` >> (
     FULL_SIMP_TAC (std_ss++holBACore_ss) []
   ) >> (
@@ -1202,11 +1198,11 @@ REPEAT STRIP_TAC >| [
     cheat
   ),
 
-  FULL_SIMP_TAC std_ss [bir_model_is_weak],
+  FULL_SIMP_TAC std_ss [bir_ts_first_enc],
 
-  FULL_SIMP_TAC std_ss [abstract_simp_jgmt_def] >>
-  FULL_SIMP_TAC (std_ss++bir_wm_SS) [abstract_jgmt_def,
-				     bir_etl_wm_def, bir_weak_trs_def] >>
+  FULL_SIMP_TAC std_ss [t_ext_jgmt_def] >>
+  FULL_SIMP_TAC (std_ss++bir_wm_SS) [t_jgmt_def,
+				     bir_ts_def, bir_weak_trs_def] >>
   REPEAT STRIP_TAC >>
   IMP_RES_TAC bir_exec_to_labels_triple_precond_subprogram >>
   QSPECL_X_ASSUM ``!s. _`` [`s`] >>
@@ -1215,7 +1211,7 @@ REPEAT STRIP_TAC >| [
 					bir_exec_to_labels_triple_precond_def] >>
   irule bir_env_oldTheory.bir_env_vars_are_initialised_ORDER >>
   Q.EXISTS_TAC `s.bst_environ` >>
-  Cases_on `bir_exec_to_labels (wl UNION bl) prog1 s` >> (
+  Cases_on `bir_exec_to_labels (il UNION el) prog1 s` >> (
     FULL_SIMP_TAC (std_ss++holBACore_ss) []
   ) >>
   FULL_SIMP_TAC std_ss [bir_exec_to_labels_def] >>
